Prove most of Spawn/JoinHandle

new/proof/std.v
@@ -1,7 +1,7 @@
 From New.proof Require Import proof_prelude.
 From New.code.github_com.goose_lang Require Import std.
 Require Export New.generatedproof.github_com.goose_lang.std.
-From New.proof Require Import primitive.
+From New.proof Require Import primitive sync.
 
 Section wps.
 Context `{hG: heapGS Σ, !ffi_semantics _ _}.
@@ -65,4 +65,138 @@ Proof.
   iIntros (?). wp_pures. do 2 wp_load. wp_pures.
   iApply "HΦ". iPureIntro. done.
 Qed.
+
+Definition is_JoinHandle (l: loc) (P: iProp Σ): iProp _ :=
+  ∃ (mu_l cond_l: loc),
+  "#mu" ∷ l ↦s[std.JoinHandle :: "mu"]□ mu_l ∗
+  "#cond" ∷ l ↦s[std.JoinHandle :: "cond"]□ cond_l ∗
+  "#Hcond" ∷ is_Cond cond_l (interface.mk sync.pkg_name' "Mutex'ptr"%go #mu_l) ∗
+  "#Hlock" ∷ is_Mutex mu_l
+     (∃ (done_b: bool),
+         "done_b" ∷ l ↦s[std.JoinHandle :: "done"] done_b ∗
+         "HP" ∷ if done_b then P else True)
+.
+
+Lemma wp_newJoinHandle (P: iProp Σ) :
+  {{{ is_initialized ∗ sync.is_initialized }}}
+    func_call #std.pkg_name' #"newJoinHandle" #()
+  {{{ (l: loc), RET #l; is_JoinHandle l P }}}.
+Proof.
+  iIntros (Φ) "[#Hi #?] HΦ". iNamed "Hi". wp_func_call. wp_call.
+  wp_alloc mu_l as "mu"; wp_pures.
+  wp_alloc m as "m"; wp_pures.
+  wp_store; wp_pures.
+  wp_alloc cond_l as "cond"; repeat (wp_load || wp_pures).
+  wp_apply (wp_NewCond with "[#]").
+  { iFrame "#". }
+  iIntros (cond) "#His_cond".
+  repeat (wp_pures || wp_store || wp_load).
+  iMod (typed_pointsto_persist with "mu") as "mu".
+  iMod (typed_pointsto_persist with "cond") as "cond".
+  wp_alloc jh_l as "jh".
+  iApply struct_fields_split in "jh". simpl. iNamed "jh".
+  iMod (typed_pointsto_persist with "Hmu") as "Hmu".
+  iMod (typed_pointsto_persist with "Hcond") as "Hcond".
+  iMod (init_Mutex (∃ (done_b: bool),
+         "done_b" ∷ jh_l ↦s[std.JoinHandle :: "done"] done_b ∗
+         "HP" ∷ if done_b then P else True)
+         with "[//] m [Hdone]") as "Hlock".
+  { iNext.
+    iFrame.
+  }
+  wp_pures.
+  iApply "HΦ".
+  rewrite /is_JoinHandle.
+  iFrame "His_cond". iFrame.
+Qed.
+
+Lemma wp_JoinHandle__finish l (P: iProp Σ) :
+  {{{ is_initialized ∗ sync.is_defined ∗ atomic.is_initialized ∗ is_JoinHandle l P ∗ P }}}
+    method_call #std.pkg_name' #"JoinHandle'ptr" #"finish" #l #()
+  {{{ RET #(); True }}}.
+Proof.
+  iIntros (Φ) "Hpre HΦ".
+  iDestruct "Hpre" as "(#init & #? & #? & #Hhandle & P)". iNamed "init".
+  iNamed "Hhandle".
+  wp_method_call. wp_call.
+  wp_alloc h_l as "h". repeat (wp_pures || wp_load).
+  wp_apply (wp_Mutex__Lock with "Hlock").
+  iIntros "[locked Hinv]". iNamed "Hinv".
+  repeat (wp_pures || wp_load || wp_store).
+  wp_apply (wp_Cond__Signal with "[$Hcond]").
+  { iFrame "#". }
+  repeat (wp_pures || wp_load).
+  wp_apply (wp_Mutex__Unlock with "[$Hlock $locked done_b P]").
+  { iFrame "done_b P". }
+  wp_pures.
+  iApply "HΦ".
+  done.
+Qed.
+
+Lemma wp_Spawn (P: iProp Σ) (f x: binder) (e: val) :
+  {{{ is_initialized ∗ sync.is_defined ∗ atomic.is_initialized ∗
+        (∀ Φ, ▷(P -∗ Φ #()) -∗ WP #({| func.f := f; func.x := x; func.e := e |}) #() {{ Φ }}) }}}
+  func_call #std.pkg_name' #"Spawn" #({| func.f := f; func.x := x; func.e := e |})
+  {{{ (l: loc), RET #l; is_JoinHandle l P }}}.
+Proof.
+  iIntros (Φ) "(#init & #? & #? & Hwp) HΦ". iNamed "init".
+  wp_func_call; wp_call.
+  wp_alloc f_l as "f"; wp_pures.
+  wp_alloc h_l as "h"; wp_pures.
+  iMod (typed_pointsto_persist with "f") as "#f".
+  wp_apply (wp_newJoinHandle P).
+  { iFrame "#". }
+  iIntros (l) "#Hhandle".
+  repeat (wp_load || wp_store || wp_pures).
+  iMod (typed_pointsto_persist with "h") as "#h".
+  wp_bind (Fork _).
+  iApply (wp_fork with "[Hwp]").
+  - iModIntro. wp_pures. wp_load.
+    (* NOTE: it's important not to do a pure reduction here since it would
+    produce a substitution into the lambda *)
+    wp_apply "Hwp".
+    iIntros "HP".
+    wp_pures. wp_load.
+    wp_apply (wp_JoinHandle__finish with "[$Hhandle $HP]").
+    { iFrame "#". }
+    wp_pures.
+    done.
+  - iModIntro.
+    repeat (wp_pures || wp_load).
+    iApply "HΦ".
+    iFrame "#".
+Qed.
+
+Lemma wp_JoinHandle__Join l P :
+  {{{ is_initialized ∗ sync.is_defined ∗ is_JoinHandle l P }}}
+    method_call #std.pkg_name' #"JoinHandle'ptr" #"Join" #l #()
+  {{{ RET #(); P }}}.
+Proof.
+  iIntros (Φ) "(#init & #? & Hjh) HΦ". iNamed "init". iNamed "Hjh".
+  wp_method_call. wp_call.
+  wp_alloc h_l as "h"; wp_pures.
+  repeat (wp_load || wp_pures).
+  wp_apply (wp_Mutex__Lock with "Hlock").
+  iIntros "[Hlocked Hlinv]". iNamed "Hlinv".
+  wp_pures.
+
+  iAssert (∃ (done_b: bool),
+           "locked" ∷ own_Mutex mu_l ∗
+           "done" ∷ l ↦s[std.JoinHandle::"done"] done_b ∗
+           "HP" ∷ (if done_b then P else True))%I
+          with "[$Hlocked $done_b $HP]" as "HI".
+  wp_for. iNamed "HI". wp_pures.
+  rewrite decide_True //.
+  repeat (wp_pures || wp_load).
+  destruct done_b0; repeat (wp_pures || wp_load || wp_store).
+  - admit. (* TODO: this isn't any of the loop terminating values, is there a translation bug? *)
+  - wp_apply (wp_Cond__Wait with "[$Hcond locked done HP]").
+      { iSplit.
+        - iApply (Mutex_is_Locker with "Hlock").
+        - iFrame. }
+      iIntros "[Hlocked Hlinv]". iNamed "Hlinv".
+      wp_pures.
+      admit. (* TODO: same as above *)
+Admitted.
+
 End wps.
